theories/lib/base.v
@@ -188,3 +188,4 @@ Proof.
   apply (elem_of_disjoint (x :: xs) ys); first done.
   apply elem_of_cons. by right.
 Qed.
+
